progs64/lock.c
@@ -1,0 +1,22 @@
+#include "lock.h"
+
+lock_t* makelock(void) {
+    return make_atomic(1);
+}
+
+void freelock(lock_t *lock) {
+    free_atomic(lock);
+}
+
+void acquire(lock_t *lock) {
+    int b = 0;
+    int expected;
+    do {
+        expected = 0;
+        b = atom_CAS(lock, &expected, 1);
+    } while (b == 0);
+}
+
+void release(lock_t *lock) {
+    atom_store(lock, 0);
+}
