atomics/SC_atomics.v
@@ -1,10 +1,10 @@
+(* SC atomics without importing Iris *)
+
+Require Import Ensembles.
 Require Import VST.veric.rmaps.
 Require Import VST.veric.compcert_rmaps.
 Require Import VST.concurrency.ghosts.
 Require Import VST.concurrency.conclib.
-Require Export VST.concurrency.invariants.
-Require Export VST.concurrency.fupd.
-Require Export VST.atomics.general_atomics.
 Require Import VST.floyd.library.
 Require Import VST.zlist.sublist.
 
@@ -75,16 +75,16 @@ Definition free_atomic_int_spec :=
     SEP ().
 
 Definition AL_type := ProdType (ProdType (ProdType (ConstType val)
-  (ConstType coPset)) (ConstType coPset))
+  (ConstType (Ensemble nat))) (ConstType (Ensemble nat)))
   (ArrowType (ConstType val) Mpred).
 
 Program Definition atomic_load_spec := TYPE AL_type
-  WITH p : val, Eo : coPset, Ei : coPset, Q : val -> mpred
+  WITH p : val, Eo : Ensemble nat, Ei : Ensemble nat, Q : val -> mpred
   PRE [ tptr atomic_int ]
-   PROP (subseteq Ei Eo)
+   PROP (Included Ei Eo)
    PARAMS (p)
    SEP (|={Eo,Ei}=> EX sh : share, EX v : val, !!(readable_share sh) &&
-              atomic_int_at sh v p * (atomic_int_at sh v p -* |={Ei,Eo}=> Q v))%I
+              atomic_int_at sh v p * (atomic_int_at sh v p -* |={Ei,Eo}=> Q v))
   POST [ tint ]
    EX v : val,
    PROP ()
@@ -93,32 +93,35 @@ Program Definition atomic_load_spec := TYPE AL_type
 Next Obligation.
 Proof.
   repeat intro.
-  unfold PROPx, PARAMSx, SEPx; simpl; rewrite !approx_andp; f_equal;
-    f_equal; rewrite -> !sepcon_emp, ?approx_sepcon, ?approx_idem.
-  setoid_rewrite fupd_nonexpansive; do 3 f_equal.
+  destruct x as (((?, ?), ?), ?).
+  unfold PROPx, PARAMSx, GLOBALSx, LOCALx, SEPx, argsassert2assert; simpl; rewrite !approx_andp; f_equal;
+    f_equal; f_equal; rewrite -> !sepcon_emp, ?approx_sepcon, ?approx_idem.
+  setoid_rewrite fupd_nonexpansive; do 2 f_equal.
   rewrite !approx_exp; apply f_equal; extensionality sh.
   rewrite !approx_exp; apply f_equal; extensionality v.
   rewrite !approx_sepcon; f_equal.
-  setoid_rewrite fview_shift_nonexpansive; rewrite approx_idem; auto.
+  setoid_rewrite wand_nonexpansive_r; f_equal; f_equal.
+  apply fupd_nonexpansive.
 Qed.
 Next Obligation.
 Proof.
   repeat intro.
+  destruct x as (((?, ?), ?), ?); simpl.
   rewrite !approx_exp; apply f_equal; extensionality v.
   unfold PROPx, LOCALx, SEPx; simpl; rewrite !approx_andp; do 2 apply f_equal;
     rewrite -> !sepcon_emp, ?approx_sepcon, ?approx_idem; auto.
 Qed.
 
 Definition AS_type := ProdType (ProdType (ProdType (ConstType (val * val))
-  (ConstType coPset)) (ConstType coPset)) Mpred.
+  (ConstType (Ensemble nat))) (ConstType (Ensemble nat))) Mpred.
 
 Program Definition atomic_store_spec := TYPE AS_type
-  WITH p : val, v : val, Eo : coPset, Ei : coPset, Q : mpred
+  WITH p : val, v : val, Eo : Ensemble nat, Ei : Ensemble nat, Q : mpred
   PRE [ tptr atomic_int, tint ]
-   PROP (subseteq Ei Eo)
+   PROP (Included Ei Eo)
    PARAMS (p; v)
    SEP (|={Eo,Ei}=> EX sh : share, !!(writable_share sh) && atomic_int_at sh Vundef p *
-      (atomic_int_at sh v p -* |={Ei,Eo}=> Q))%I
+      (atomic_int_at sh v p -* |={Ei,Eo}=> Q))
   POST [ tvoid ]
    PROP ()
    LOCAL ()
@@ -126,32 +129,35 @@ Program Definition atomic_store_spec := TYPE AS_type
 Next Obligation.
 Proof.
   repeat intro.
-  unfold PROPx, PARAMSx, SEPx; simpl; rewrite !approx_andp; f_equal;
-    f_equal; rewrite -> !sepcon_emp, ?approx_sepcon, ?approx_idem.
-  setoid_rewrite fupd_nonexpansive; do 3 f_equal.
+  destruct x as ((((?, ?), ?), ?), ?).
+  unfold PROPx, PARAMSx, GLOBALSx, LOCALx, SEPx, argsassert2assert; simpl; rewrite !approx_andp; f_equal;
+    f_equal; f_equal; rewrite -> !sepcon_emp, ?approx_sepcon, ?approx_idem.
+  setoid_rewrite fupd_nonexpansive; do 2 f_equal.
   rewrite !approx_exp; apply f_equal; extensionality sh.
   rewrite !approx_sepcon; f_equal.
-  setoid_rewrite fview_shift_nonexpansive; rewrite approx_idem; auto.
+  setoid_rewrite wand_nonexpansive_r; f_equal; f_equal.
+  apply fupd_nonexpansive.
 Qed.
 Next Obligation.
 Proof.
   repeat intro.
+  destruct x as ((((?, ?), ?), ?), ?); simpl.
   unfold PROPx, LOCALx, SEPx; simpl; rewrite !approx_andp; do 2 apply f_equal;
     rewrite -> !sepcon_emp, ?approx_sepcon, ?approx_idem; auto.
 Qed.
 
 Definition ACAS_type := ProdType (ProdType (ProdType (ConstType (val * share * val * val * val))
-  (ConstType coPset)) (ConstType coPset))
+  (ConstType (Ensemble nat))) (ConstType (Ensemble nat)))
   (ArrowType (ConstType val) Mpred).
 
 Program Definition atomic_CAS_spec := TYPE ACAS_type
-  WITH p : val, shc : share, pc : val, c : val, v : val, Eo : coPset, Ei : coPset, Q : val -> mpred
+  WITH p : val, shc : share, pc : val, c : val, v : val, Eo : Ensemble nat, Ei : Ensemble nat, Q : val -> mpred
   PRE [ tptr atomic_int, tptr tint, tint ]
-   PROP (readable_share shc; subseteq Ei Eo)
+   PROP (readable_share shc; Included Ei Eo)
    PARAMS (p; pc; v)
    SEP (data_at shc tint c pc; |={Eo,Ei}=> EX sh : share, EX v0 : val,
       !!(writable_share sh) && atomic_int_at sh v0 p *
-           (atomic_int_at sh (if eq_dec v0 c then v else v0) p -* |={Ei,Eo}=> Q v0))%I
+           (atomic_int_at sh (if eq_dec v0 c then v else v0) p -* |={Ei,Eo}=> Q v0))
   POST [ tint ]
    EX v' : val,
    PROP ()
@@ -160,35 +166,38 @@ Program Definition atomic_CAS_spec := TYPE ACAS_type
 Next Obligation.
 Proof.
   repeat intro.
-  unfold PROPx, PARAMSx, SEPx; simpl; rewrite !approx_andp; f_equal;
-    f_equal; rewrite -> !sepcon_emp, ?approx_sepcon, ?approx_idem.
-  unfold argsassert2assert; rewrite !approx_sepcon; do 2 f_equal.
+  destruct x as (((((((?, ?), ?), ?), ?), ?), ?), ?).
+  unfold PROPx, PARAMSx, GLOBALSx, LOCALx, SEPx, argsassert2assert; simpl; rewrite !approx_andp; f_equal;
+    f_equal; f_equal; rewrite -> !sepcon_emp, ?approx_sepcon, ?approx_idem.
+  f_equal.
   setoid_rewrite fupd_nonexpansive; do 2 f_equal.
   rewrite !approx_exp; apply f_equal; extensionality sh.
-  rewrite !approx_exp; apply f_equal; extensionality v2.
+  rewrite !approx_exp; apply f_equal; extensionality.
   rewrite !approx_sepcon; f_equal.
-  setoid_rewrite fview_shift_nonexpansive; rewrite approx_idem; auto.
+  setoid_rewrite wand_nonexpansive_r; f_equal; f_equal.
+  apply fupd_nonexpansive.
 Qed.
 Next Obligation.
 Proof.
   repeat intro.
+  destruct x as (((((((?, ?), ?), ?), ?), ?), ?), ?); simpl.
   rewrite !approx_exp; apply f_equal; extensionality vr.
   unfold PROPx, LOCALx, SEPx; simpl; rewrite !approx_andp; do 2 apply f_equal;
     rewrite -> !sepcon_emp, ?approx_sepcon, ?approx_idem; auto.
 Qed.
 
 Definition AEX_type := ProdType (ProdType (ProdType (ConstType (val * val))
-  (ConstType coPset)) (ConstType coPset))
+  (ConstType (Ensemble nat))) (ConstType (Ensemble nat)))
   (ArrowType (ConstType val) Mpred).
 
 Program Definition atomic_exchange_spec := TYPE AEX_type
-  WITH p : val, v : val, Eo : coPset, Ei : coPset, Q : val -> mpred
+  WITH p : val, v : val, Eo : Ensemble nat, Ei : Ensemble nat, Q : val -> mpred
   PRE [ tptr tint, tint ]
-   PROP (subseteq Ei Eo)
+   PROP (Included Ei Eo)
    PARAMS (p; v)
    SEP (|={Eo,Ei}=> EX sh : share, EX v0 : val, !!(writable_share sh) &&
               data_at sh tint v0 p *
-        (data_at sh tint v p -* |={Ei,Eo}=> Q v0))%I
+        (data_at sh tint v p -* |={Ei,Eo}=> Q v0))
   POST [ tint ]
    EX v' : val,
    PROP ()
@@ -197,413 +206,20 @@ Program Definition atomic_exchange_spec := TYPE AEX_type
 Next Obligation.
 Proof.
   repeat intro.
-  unfold PROPx, PARAMSx, SEPx; simpl; rewrite !approx_andp; f_equal;
-    f_equal; rewrite -> !sepcon_emp, ?approx_sepcon, ?approx_idem.
-  unfold argsassert2assert; f_equal.
+  destruct x as ((((?, ?), ?), ?), ?).
+  unfold PROPx, PARAMSx, GLOBALSx, LOCALx, SEPx, argsassert2assert; simpl; rewrite !approx_andp; f_equal;
+    f_equal; f_equal; rewrite -> !sepcon_emp, ?approx_sepcon, ?approx_idem.
   setoid_rewrite fupd_nonexpansive; do 2 f_equal.
   rewrite !approx_exp; apply f_equal; extensionality sh.
-  rewrite !approx_exp; apply f_equal; extensionality v0.
+  rewrite !approx_exp; apply f_equal; extensionality.
   rewrite !approx_sepcon; f_equal.
-  setoid_rewrite fview_shift_nonexpansive; rewrite approx_idem; auto.
+  setoid_rewrite wand_nonexpansive_r; f_equal; f_equal.
+  apply fupd_nonexpansive.
 Qed.
 Next Obligation.
 Proof.
   repeat intro.
-  rewrite !approx_exp; apply f_equal; extensionality vr.
-  unfold PROPx, LOCALx, SEPx; simpl; rewrite !approx_andp; do 2 apply f_equal;
-    rewrite -> !sepcon_emp, ?approx_sepcon, ?approx_idem; auto.
-Qed.
-
-(* subspecs for integer operations *)
-Definition ALI_type := ProdType (ProdType (ProdType (ConstType val)
-  (ConstType coPset)) (ConstType coPset))
-  (ArrowType (ConstType Z) Mpred).
-
-Program Definition atomic_load_int_spec := TYPE ALI_type
-  WITH p : val, Eo : coPset, Ei : coPset, Q : Z -> mpred
-  PRE [ tptr atomic_int ]
-   PROP (subseteq Ei Eo)
-   PARAMS (p)
-   SEP (|={Eo,Ei}=> EX sh : share, EX v : Z, !!(readable_share sh /\ repable_signed v) &&
-              atomic_int_at sh (vint v) p * (atomic_int_at sh (vint v) p -* |={Ei,Eo}=> Q v))%I
-  POST [ tint ]
-   EX v : Z,
-   PROP (repable_signed v)
-   LOCAL (temp ret_temp (vint v))
-   SEP (Q v).
-Next Obligation.
-Proof.
-  repeat intro.
-  unfold PROPx, LOCALx, SEPx; simpl; rewrite !approx_andp; f_equal;
-    f_equal; rewrite -> !sepcon_emp, ?approx_sepcon, ?approx_idem.
-  setoid_rewrite fupd_nonexpansive; do 3 f_equal.
-  rewrite !approx_exp; apply f_equal; extensionality sh.
-  rewrite !approx_exp; apply f_equal; extensionality v.
-  rewrite !approx_sepcon; f_equal.
-  setoid_rewrite fview_shift_nonexpansive; rewrite approx_idem; auto.
-Qed.
-Next Obligation.
-Proof.
-  repeat intro.
-  rewrite !approx_exp; apply f_equal; extensionality v.
-  unfold PROPx, LOCALx, SEPx; simpl; rewrite !approx_andp; do 2 apply f_equal;
-    rewrite -> !sepcon_emp, ?approx_sepcon, ?approx_idem; auto.
-Qed.
-
-Lemma atomic_load_int : funspec_sub atomic_load_spec atomic_load_int_spec.
-Proof.
-  apply prove_funspec_sub.
-  split; auto; intros; simpl in *.
-  destruct x2 as (((p, Eo), Ei), Q).
-  intros; iIntros "[_ H] !>".
-  iExists nil, (p, Eo, Ei, fun v => match v with Vint i => Q (Int.signed i) | _ => FF end), emp.
-  rewrite emp_sepcon; iSplit.
-  - unfold PROPx, PARAMSx, GLOBALSx, LOCALx, SEPx, argsassert2assert; simpl.
-    iDestruct "H" as "($ & $ & $ & H & $)".
-    iMod "H"; iModIntro.
-    iDestruct "H" as (sh v) "[[% H1] H2]".
-    destruct H.
-    iExists sh, (vint v); iFrame.
-    rewrite Int.signed_repr; auto.
-  - iPureIntro.
-    iIntros (?) "(_ & _ & H)".
-    unfold PROPx, LOCALx, SEPx; simpl.
-    iDestruct "H" as (r) "(_ & % & Q & _)".
-    destruct H, r; try done.
-    iExists (Int.signed i); iSplit; auto.
-    { iPureIntro; split; auto.
-      apply Int.signed_range. }
-    iSplit; [iSplit; auto|].
-    { rewrite Int.repr_signed; auto. }
-    rewrite sepcon_emp; auto.
-Qed.
-
-Definition ASI_type := ProdType (ProdType (ProdType (ConstType (val * Z))
-  (ConstType coPset)) (ConstType coPset)) Mpred.
-
-Program Definition atomic_store_int_spec := TYPE ASI_type
-  WITH p : val, v : Z, Eo : coPset, Ei : coPset, Q : mpred
-  PRE [ tptr atomic_int, tint ]
-   PROP (repable_signed v; subseteq Ei Eo)
-   PARAMS (p; vint v)
-   SEP (|={Eo,Ei}=> EX sh : share, !!(writable_share sh) && atomic_int_at sh Vundef p *
-      (atomic_int_at sh (vint v) p -* |={Ei,Eo}=> Q))%I
-  POST [ tvoid ]
-   PROP ()
-   LOCAL ()
-   SEP (Q).
-Next Obligation.
-Proof.
-  repeat intro.
-  unfold PROPx, LOCALx, SEPx; simpl; rewrite !approx_andp; f_equal;
-    f_equal; rewrite -> !sepcon_emp, ?approx_sepcon, ?approx_idem.
-  setoid_rewrite fupd_nonexpansive; do 3 f_equal.
-  rewrite !approx_exp; apply f_equal; extensionality sh.
-  rewrite !approx_sepcon; f_equal.
-  setoid_rewrite fview_shift_nonexpansive; rewrite approx_idem; auto.
-Qed.
-Next Obligation.
-Proof.
-  repeat intro.
-  unfold PROPx, LOCALx, SEPx; simpl; rewrite !approx_andp; do 2 apply f_equal;
-    rewrite -> !sepcon_emp, ?approx_sepcon, ?approx_idem; auto.
-Qed.
-
-Lemma atomic_store_int : funspec_sub atomic_store_spec atomic_store_int_spec.
-Proof.
-  apply prove_funspec_sub.
-  split; auto; intros; simpl in *.
-  destruct x2 as ((((p, v), Eo), Ei), Q).
-  intros; iIntros "[_ H] !>".
-  iExists nil, (p, vint v, Eo, Ei, Q), emp.
-  rewrite emp_sepcon; iSplit.
-  - unfold PROPx, PARAMSx, GLOBALSx, LOCALx, SEPx; simpl.
-    iDestruct "H" as "(% & $ & $ & H & $)".
-    destruct H; auto.
-  - iPureIntro.
-    by iIntros (?) "(_ & _ & $)".
-Qed.
-
-Definition ACASI_type := ProdType (ProdType (ProdType (ConstType (val * share * val * Z * Z))
-  (ConstType coPset)) (ConstType coPset))
-  (ArrowType (ConstType Z) Mpred).
-
-Program Definition atomic_CAS_int_spec := TYPE ACASI_type
-  WITH p : val, shc : share, pc : val, c : Z, v : Z, Eo : coPset, Ei : coPset, Q : Z -> mpred
-  PRE [ tptr atomic_int, tptr tint, tint ]
-   PROP (repable_signed c; repable_signed v; readable_share shc; subseteq Ei Eo)
-   PARAMS (p; pc; vint v)
-   SEP (data_at shc tint (vint c) pc; |={Eo,Ei}=> EX sh : share, EX v0 : Z,
-      !!(writable_share sh /\ repable_signed v0) && atomic_int_at sh (vint v0) p *
-           (atomic_int_at sh (vint (if eq_dec v0 c then v else v0)) p -* |={Ei,Eo}=> Q v0))%I
-  POST [ tint ]
-   EX v' : Z,
-   PROP (repable_signed v')
-   LOCAL (temp ret_temp (vint (if eq_dec v' c then 1 else 0)))
-   SEP (data_at shc tint (vint v') pc; Q v').
-Next Obligation.
-Proof.
-  repeat intro.
-  unfold PROPx, LOCALx, SEPx; simpl; rewrite !approx_andp; f_equal;
-    f_equal; rewrite -> !sepcon_emp, ?approx_sepcon, ?approx_idem.
-  unfold argsassert2assert; rewrite !approx_sepcon; do 2 f_equal.
-  setoid_rewrite fupd_nonexpansive; do 2 f_equal.
-  rewrite !approx_exp; apply f_equal; extensionality sh.
-  rewrite !approx_exp; apply f_equal; extensionality v2.
-  rewrite !approx_sepcon; f_equal.
-  setoid_rewrite fview_shift_nonexpansive; rewrite approx_idem; auto.
-Qed.
-Next Obligation.
-Proof.
-  repeat intro.
-  rewrite !approx_exp; apply f_equal; extensionality vr.
-  unfold PROPx, LOCALx, SEPx; simpl; rewrite !approx_andp; do 2 apply f_equal;
-    rewrite -> !sepcon_emp, ?approx_sepcon, ?approx_idem; auto.
-Qed.
-
-Lemma atomic_CAS_int : funspec_sub atomic_CAS_spec atomic_CAS_int_spec.
-Proof.
-  apply prove_funspec_sub.
-  split; auto; intros; simpl in *.
-  destruct x2 as (((((((p, shc), pc), c), v), Eo), Ei), Q).
-  intros; iIntros "[_ H] !>".
-  iExists nil, (p, shc, pc, vint c, vint v, Eo, Ei, fun v => match v with Vint i => Q (Int.signed i) | _ => FF end), emp.
-  rewrite emp_sepcon; iSplit.
-  - unfold PROPx, PARAMSx, GLOBALSx, LOCALx, SEPx; simpl.
-    iDestruct "H" as "(% & $ & $ & $ & H & $)".
-    destruct H as (? & ? & ?); iSplit; auto.
-    iMod "H"; iModIntro.
-    iDestruct "H" as (sh v0) "[[% H1] H2]".
-    destruct H2.
-    iExists sh, (vint v0); iFrame.
-    rewrite -> Int.signed_repr by auto.
-    iSplit; first done.
-    if_tac.
-    + subst; rewrite eq_dec_refl; done.
-    + if_tac; last done.
-      match goal with H : vint _ = vint _ |- _ => apply Vint_inj, repr_inj_signed in H end; auto; contradiction.
-  - unfold PROPx, LOCALx, SEPx; simpl.
-    iDestruct "H" as "[% _]".
-    destruct H as [Hc _].
-    iPureIntro.
-    iIntros (?) "(_ & _ & H)".
-    iDestruct "H" as (r) "(_ & % & ? & Q & _)".
-    destruct H, r; try done.
-    iExists (Int.signed i); iSplit; auto.
-    { iPureIntro; split; auto.
-      apply Int.signed_range. }
-    iSplit; [iSplit; auto|].
-    { if_tac; if_tac in H; auto; subst.
-      + rewrite Int.repr_signed in H2; contradiction.
-      + apply Vint_inj in H2; subst.
-        rewrite -> Int.signed_repr in H1 by auto; contradiction. }
-    rewrite Int.repr_signed sepcon_emp; iFrame.
-Qed.
-
-Definition AEXI_type := ProdType (ProdType (ProdType (ConstType (val * Z))
-  (ConstType coPset)) (ConstType coPset))
-  (ArrowType (ConstType Z) Mpred).
-
-Program Definition atomic_exchange_int_spec := TYPE AEXI_type
-  WITH p : val, v : Z, Eo : coPset, Ei : coPset, Q : Z -> mpred
-  PRE [ tptr tint, tint ]
-   PROP (repable_signed v; subseteq Ei Eo)
-   PARAMS (p; vint v)
-   SEP (|={Eo,Ei}=> EX sh : share, EX v0 : Z, !!(writable_share sh /\ repable_signed v0) &&
-              data_at sh tint (vint v0) p *
-        (data_at sh tint (vint v) p -* |={Ei,Eo}=> Q v0))%I
-  POST [ tint ]
-   EX v' : Z,
-   PROP (repable_signed v')
-   LOCAL (temp ret_temp (vint v'))
-   SEP (Q v').
-Next Obligation.
-Proof.
-  repeat intro.
-  unfold PROPx, LOCALx, SEPx; simpl; rewrite !approx_andp; f_equal;
-    f_equal; rewrite -> !sepcon_emp, ?approx_sepcon, ?approx_idem.
-  setoid_rewrite fupd_nonexpansive; do 3 f_equal.
-  rewrite !approx_exp; apply f_equal; extensionality sh.
-  rewrite !approx_exp; apply f_equal; extensionality v0.
-  rewrite !approx_sepcon; f_equal.
-  setoid_rewrite fview_shift_nonexpansive; rewrite approx_idem; auto.
-Qed.
-Next Obligation.
-Proof.
-  repeat intro.
-  rewrite !approx_exp; apply f_equal; extensionality vr.
-  unfold PROPx, LOCALx, SEPx; simpl; rewrite !approx_andp; do 2 apply f_equal;
-    rewrite -> !sepcon_emp, ?approx_sepcon, ?approx_idem; auto.
-Qed.
-
-Lemma atomic_exchange_int : funspec_sub atomic_exchange_spec atomic_exchange_int_spec.
-Proof.
-  apply prove_funspec_sub.
-  split; auto; intros; simpl in *.
-  destruct x2 as ((((p, v), Eo), Ei), Q).
-  intros; iIntros "[_ H] !>".
-  iExists nil, (p, vint v, Eo, Ei, fun v => match v with Vint i => Q (Int.signed i) | _ => FF end), emp.
-  rewrite emp_sepcon; iSplit.
-  - unfold PROPx, PARAMSx, GLOBALSx, LOCALx, SEPx; simpl.
-    iDestruct "H" as "(% & $ & $ & H & $)".
-    destruct H; iSplit; auto.
-    iMod "H"; iModIntro.
-    iDestruct "H" as (sh v0) "[[% H1] H2]".
-    destruct H1.
-    iExists sh, (vint v0); iFrame.
-    rewrite -> Int.signed_repr; auto.
-  - unfold PROPx, LOCALx, SEPx; simpl.
-    iPureIntro.
-    iIntros (?) "(_ & _ & H)".
-    iDestruct "H" as (r) "(_ & % & Q & _)".
-    destruct H, r; try done.
-    iExists (Int.signed i); iSplit; auto.
-    { iPureIntro; split; auto.
-      apply Int.signed_range. }
-    iSplit; [iSplit; auto|].
-    { rewrite Int.repr_signed; auto. }
-    rewrite sepcon_emp; iFrame.
-Qed.
-
-(* specs for pointer operations *)
-
-Definition ALI_ptr_type := ProdType (ProdType (ProdType (ConstType val)
-  (ConstType coPset)) (ConstType coPset))
-  (ArrowType (ConstType val) Mpred).
-
-Program Definition atomic_load_ptr_spec := TYPE ALI_ptr_type
-  WITH p : val, Eo : coPset, Ei : coPset, Q : val -> mpred
-  PRE [ tptr atomic_ptr ]
-   PROP (subseteq Ei Eo)
-   PARAMS (p)
-   SEP (|={Eo,Ei}=> EX sh : share, EX v : val, !!(readable_share sh ) &&
-              atomic_ptr_at sh v p * (atomic_ptr_at sh v p -* |={Ei,Eo}=> Q v))%I
-  POST [ tptr Tvoid ]
-   EX v : val,
-   PROP ()
-   LOCAL (temp ret_temp v)
-   SEP (Q v).
-Next Obligation.
-Proof.
-  repeat intro.
-  unfold PROPx, LOCALx, SEPx; simpl; rewrite !approx_andp; f_equal;
-    f_equal; rewrite -> !sepcon_emp, ?approx_sepcon, ?approx_idem.
-  setoid_rewrite fupd_nonexpansive; do 3 f_equal.
-  rewrite !approx_exp; apply f_equal; extensionality sh.
-  rewrite !approx_exp; apply f_equal; extensionality v.
-  rewrite !approx_sepcon; f_equal.
-  setoid_rewrite fview_shift_nonexpansive; rewrite approx_idem; auto.
-Qed.
-Next Obligation.
-Proof.
-  repeat intro.
-  rewrite !approx_exp; apply f_equal; extensionality v.
-  unfold PROPx, LOCALx, SEPx; simpl; rewrite !approx_andp; do 2 apply f_equal;
-    rewrite -> !sepcon_emp, ?approx_sepcon, ?approx_idem; auto.
-Qed.
-
-
-Definition ASI_ptr_type := ProdType (ProdType (ProdType (ConstType (val * val))
-  (ConstType coPset)) (ConstType coPset)) Mpred.
-
-Program Definition atomic_store_ptr_spec := TYPE ASI_ptr_type
-  WITH p : val, v : val, Eo : coPset, Ei : coPset, Q : mpred
-  PRE [ tptr atomic_ptr, tptr Tvoid ]
-   PROP (subseteq Ei Eo)
-   PARAMS (p; v)
-   SEP (|={Eo,Ei}=> EX sh : share, !!(writable_share sh) && atomic_ptr_at sh Vundef p *
-      (atomic_ptr_at sh v p -* |={Ei,Eo}=> Q))%I
-  POST [ tvoid ]
-   PROP ()
-   LOCAL ()
-   SEP (Q).
-Next Obligation.
-Proof.
-  repeat intro.
-  unfold PROPx, LOCALx, SEPx; simpl; rewrite !approx_andp; f_equal;
-    f_equal; rewrite -> !sepcon_emp, ?approx_sepcon, ?approx_idem.
-  setoid_rewrite fupd_nonexpansive; do 3 f_equal.
-  rewrite !approx_exp; apply f_equal; extensionality sh.
-  rewrite !approx_sepcon; f_equal.
-  setoid_rewrite fview_shift_nonexpansive; rewrite approx_idem; auto.
-Qed.
-Next Obligation.
-Proof.
-  repeat intro.
-  unfold PROPx, LOCALx, SEPx; simpl; rewrite !approx_andp; do 2 apply f_equal;
-    rewrite -> !sepcon_emp, ?approx_sepcon, ?approx_idem; auto.
-Qed.
-
-
-Definition ACASI_ptr_type := ProdType (ProdType (ProdType (ConstType (val * share * val * val * val))
-  (ConstType coPset)) (ConstType coPset))
-  (ArrowType (ConstType val) Mpred).
-
-Program Definition atomic_CAS_ptr_spec := TYPE ACASI_ptr_type
-  WITH p : val, shc : share, pc : val, c : val, v : val, Eo : coPset, Ei : coPset, Q : val -> mpred
-  PRE [ tptr atomic_ptr, tptr (tptr Tvoid), tptr Tvoid ]
-   PROP (readable_share shc; subseteq Ei Eo)
-   PARAMS (p; pc; v)
-   SEP (data_at shc (tptr Tvoid) c pc; |={Eo,Ei}=> EX sh : share, EX v0 : val,
-      !!(writable_share sh ) && atomic_ptr_at sh v0 p *
-           (atomic_ptr_at sh (if eq_dec v0 c then v else v0) p -* |={Ei,Eo}=> Q v0))%I
-  POST [ tint ]
-   EX v' : val,
-   PROP ()
-   LOCAL (temp ret_temp (vint (if eq_dec v' c then 1 else 0)))
-   SEP (data_at shc (tptr Tvoid) c pc; Q v').
-Next Obligation.
-Proof.
-  repeat intro.
-  unfold PROPx, LOCALx, SEPx; simpl; rewrite !approx_andp; f_equal;
-    f_equal; rewrite -> !sepcon_emp, ?approx_sepcon, ?approx_idem.
-  unfold argsassert2assert; rewrite !approx_sepcon; f_equal.
-  setoid_rewrite fupd_nonexpansive; do 3 f_equal.
-  rewrite !approx_exp; apply f_equal; extensionality sh.
-  rewrite !approx_exp; apply f_equal; extensionality v2.
-  rewrite !approx_sepcon; f_equal.
-  setoid_rewrite fview_shift_nonexpansive; rewrite approx_idem; auto.
-Qed.
-Next Obligation.
-Proof.
-  repeat intro.
-  rewrite !approx_exp; apply f_equal; extensionality vr.
-  unfold PROPx, LOCALx, SEPx; simpl; rewrite !approx_andp; do 2 apply f_equal;
-    rewrite -> !sepcon_emp, ?approx_sepcon, ?approx_idem; auto.
-Qed.
-
-
-Definition AEXI_ptr_type := ProdType (ProdType (ProdType (ConstType (val * val))
-  (ConstType coPset)) (ConstType coPset))
-  (ArrowType (ConstType val) Mpred).
-
-Program Definition atomic_exchange_ptr_spec := TYPE AEXI_ptr_type
-  WITH p : val, v : val, Eo : coPset, Ei : coPset, Q : val -> mpred
-  PRE [ tptr atomic_ptr, tptr Tvoid ]
-   PROP (subseteq Ei Eo)
-   PARAMS (p; v)
-   SEP (|={Eo,Ei}=> EX sh : share, EX v0 : val, !!(writable_share sh ) &&
-              atomic_ptr_at sh v0 p *
-        (atomic_ptr_at sh v p -* |={Ei,Eo}=> Q v0))%I
-  POST [ tint ]
-   EX v' : val,
-   PROP ()
-   LOCAL (temp ret_temp v')
-   SEP (Q v').
-Next Obligation.
-Proof.
-  repeat intro.
-  unfold PROPx, LOCALx, SEPx; simpl; rewrite !approx_andp; f_equal;
-    f_equal; rewrite -> !sepcon_emp, ?approx_sepcon, ?approx_idem.
-  setoid_rewrite fupd_nonexpansive; do 3 f_equal.
-  rewrite !approx_exp; apply f_equal; extensionality sh.
-  rewrite !approx_exp; apply f_equal; extensionality v0.
-  rewrite !approx_sepcon; f_equal.
-  setoid_rewrite fview_shift_nonexpansive; rewrite approx_idem; auto.
-Qed.
-Next Obligation.
-Proof.
-  repeat intro.
+  destruct x as ((((?, ?), ?), ?), ?); simpl.
   rewrite !approx_exp; apply f_equal; extensionality vr.
   unfold PROPx, LOCALx, SEPx; simpl; rewrite !approx_andp; do 2 apply f_equal;
     rewrite -> !sepcon_emp, ?approx_sepcon, ?approx_idem; auto.
