concurrency/cancelable_invariants.v
@@ -1,0 +1,161 @@
+(* recapitulate iris/base_logic/lib/cancelable_invariants.v *)
+Require Import VST.msl.shares.
+Require Import VST.veric.shares.
+Require Import VST.msl.ghost.
+Require Import VST.msl.ghost_seplog.
+Require Import VST.veric.invariants.
+Require Import VST.concurrency.conclib.
+
+#[export] Program Instance share_ghost : Ghost := { G := share; valid _ := True }.
+
+Definition cinv_own g sh := own(RA := share_ghost) g sh compcert_rmaps.RML.R.NoneP.
+
+Definition cinvariant i g P := invariant i (P || cinv_own g Tsh).
+
+Lemma cinv_alloc' : forall P, wsat * |> P |-- |==> wsat * EX i : _, EX g : _, cinvariant i g P * cinv_own g Tsh.
+Proof.
+  intros.
+  rewrite <- emp_sepcon at 1.
+  eapply derives_trans; [eapply derives_trans, bupd_frame_r|].
+  { apply sepcon_derives, derives_refl.
+    apply (own_alloc(RA := share_ghost)), I. }
+  eapply derives_trans, bupd_trans; apply bupd_mono.
+  Intros g.
+  eapply derives_trans; [eapply derives_trans; [|apply sepcon_derives, derives_refl; unseal_derives; apply wsat_alloc]|].
+  2: { unseal_derives; eapply predicates_hered.derives_trans, own.bupd_mono; [apply own.bupd_frame_r|].
+       rewrite exp_sepcon2, predicates_sl.exp_sepcon2.
+       rewrite predicates_sl.exp_sepcon1.
+       apply predicates_hered.exp_derives; intros.
+       rewrite predicates_sl.sepcon_assoc.
+       apply predicates_sl.sepcon_derives; [apply predicates_hered.derives_refl|].
+       eapply predicates_hered.exp_right, predicates_hered.derives_refl. }
+  rewrite sepcon_comm; apply sepcon_derives, derives_refl.
+  change predicates_sl.sepcon with sepcon; apply sepcon_derives; [apply derives_refl|].
+  change (predicates_hered.box predicates_hered.laterM) with later; apply later_derives, orp_right1, derives_refl.
+Qed.
+
+Corollary cinv_alloc : forall E P, |> P |-- |={E}=> EX i : _, EX g : _, cinvariant i g P * cinv_own g Tsh.
+Proof.
+  intros.
+  apply wsat_fupd, cinv_alloc'.
+Qed.
+
+Lemma cinv_cancel' : forall E i g P, cinvariant i g P * cinv_own g Tsh |-- |={E}=> |> P.
+Proof.
+  intros; unfold cinvariant.
+(*  apply wsat_open.*)
+Admitted.
+
+Corollary cinv_cancel : forall E i g P, cinvariant i g P * cinv_own g Tsh |-- |={E}=> |> P.
+Proof.
+  intros.
+  apply wsat_fupd, cinv_cancel'.
+Qed.
+
+Lemma cinv_open : forall i P,
+  wsat * cinvariant i P * ghost_set g_en (Ensembles.Singleton i) |--
+  (|==> wsat * |> P * ghost_list g_dis (list_singleton i (Some tt)))%I.
+Proof.
+(* apply wsat_open. *)
+Admitted.
+
+(*Lemma wsat_close : forall i P,
+  wsat * invariant i P * |> P * ghost_list g_dis (list_singleton i (Some tt)) |--
+  (|==> wsat * ghost_set g_en (Ensembles.Singleton i))%I.
+Proof.
+  intros; unfold wsat, invariant.
+  iIntros "(((H & inv1) & HP) & dis1)". iDestruct "H" as (l lg lb) "((((% & inv) & dis) & en) & I)". iDestruct "inv1" as (g) "[snap agree]".
+  iAssert (!!(i < length lg /\ Znth (Z.of_nat i) lg = g /\
+    exists b, Znth (Z.of_nat i) lb = Some b)%nat) as %Hi.
+  { iCombine "snap inv" as "inv"; unfold master_list; erewrite snap_master_join1.
+    iDestruct "inv" as "[% inv]".
+    apply list_incl_singleton in H0.
+    destruct (lt_dec i (length lg));
+      [|erewrite nth_overflow in H0 by (erewrite map_length, upto_length; lia); discriminate].
+    erewrite nth_map' with (d' := 0) in H0 by (rewrite upto_length; lia).
+    erewrite nth_upto in H0 by lia.
+    destruct (Znth (Z.of_nat i) lb); inv H0; eauto. }
+  iDestruct "snap" as "_".
+  iModIntro.
+  destruct Hi as (? & ? & b & Hi).
+  assert (nth i lb None = Some b) as Hi' by (rewrite <- nth_Znth' in Hi; auto).
+  destruct b.
+  { iCombine "dis dis1" as "dis".
+    iDestruct (own_valid_2(RA := list_PCM _) with "[$dis]") as %H2.
+    destruct H2 as (? & J & _).
+    apply list_join_nth with (n := i) in J.
+    erewrite nth_singleton, nth_map' with (d' := None) in J by lia.
+    rewrite Hi' in J; inv J.
+    inv H5.
+    inv H3. }
+  erewrite ghost_set_remove with (a := i).
+  iDestruct "en" as "[$ en]".
+  iExists l, lg, (replace_nth i lb (Some true)).
+  rewrite replace_nth_length predicates_hered.prop_true_andp; last auto.
+  iSplitR "I agree HP".
+  iSplitR "en".
+  iSplitR "dis dis1".
+  - erewrite map_ext; [iFrame|].
+    intros.
+    destruct (eq_dec a (Z.of_nat i)); [subst; rewrite Znth_replace_nth | rewrite Znth_replace_nth'];
+      auto; try lia.
+    rewrite Hi; auto.
+  - iCombine "dis1 dis" as "dis"; setoid_rewrite <- own.ghost_op; [iFrame|].
+    rewrite map_replace_nth.
+    apply (list_join_singleton(P := token_PCM)).
+    { rewrite map_length; lia. }
+    erewrite nth_map' with (d' := None) by lia.
+    rewrite Hi'; constructor.
+  - erewrite Ensembles.Extensionality_Ensembles at 1; [iFrame|]; constructor; intros ? X.
+    + inv X; unfold Ensembles.In in *.
+      rewrite nth_replace_nth'; auto.
+      intro; subst; contradiction.
+    + constructor.
+      * unfold Ensembles.In in *.
+        destruct (eq_dec x i); [subst; auto|].
+        rewrite nth_replace_nth' in X; auto.
+      * intro X'; inv X'.
+        unfold Ensembles.In in X.
+        rewrite -> nth_replace_nth in X by lia; inv X.
+  - erewrite !iter_sepcon_eq, @iter_sepcon_Znth with (i := Z.of_nat i)
+      by (rewrite Zlength_upto; split; [|apply Nat2Z.inj_lt]; lia).
+    erewrite @iter_sepcon_Znth with (i := Z.of_nat i)(l := upto _)
+      by (rewrite Zlength_upto; split; [|apply Nat2Z.inj_lt]; lia).
+    erewrite !Znth_upto, !Znth_replace_nth by lia.
+    rewrite Hi.
+    iDestruct "I" as "[agree' I]".
+    subst; iDestruct (agree_join2 with "[agree' agree]") as "[imp agree]"; first by iFrame.
+    iPoseProof ("imp" with "HP") as "?"; iFrame.
+    erewrite iter_sepcon_func_strong; eauto.
+    unfold remove_Znth; intros ? Hin.
+    rewrite Znth_replace_nth'; auto.
+    intro; subst.
+    apply in_app in Hin as [?%In_sublist_upto | ?%In_sublist_upto]; lia.
+  - unfold Ensembles.In; auto.
+Qed.*)
+
+(*Lemma cinvariant_nonexpansive : forall N, nonexpansive (cinvariant N).
+Proof.
+  intros; unfold inv.
+  apply @exists_nonexpansive; intros i.
+  apply @conj_nonexpansive, invariant_nonexpansive.
+  apply const_nonexpansive.
+Qed.
+
+Lemma inv_nonexpansive2 : forall N f, nonexpansive f ->
+  nonexpansive (fun a => inv N (f a)).
+Proof.
+  intros; unfold inv.
+  apply @exists_nonexpansive; intros i.
+  apply @conj_nonexpansive, invariant_nonexpansive2, H.
+  apply const_nonexpansive.
+Qed.*)
+
+Lemma cinvariant_super_non_expansive : forall i g R n, compcert_rmaps.RML.R.approx n (cinvariant i g R) =
+  compcert_rmaps.RML.R.approx n (cinvariant i g (compcert_rmaps.RML.R.approx n R)).
+Proof.
+  intros; unfold cinvariant.
+  rewrite invariant_super_non_expansive; setoid_rewrite invariant_super_non_expansive at 2; do 2 f_equal.
+  rewrite !approx_orp; f_equal.
+  rewrite approx_idem; auto.
+Qed.
