progs64/verif_incr.v
@@ -51,7 +51,7 @@ Definition thread_lock_inv sh g1 g2 ctr lockc lockt :=
 Definition thread_func_spec :=
  DECLARE _thread_func
   WITH y : val, x : share * gname * gname * globals
-  PRE [ tptr tvoid ]
+  PRE [ (*_args OF*) (tptr tvoid) ]
          let '(sh, g1, g2, gv) := x in
          PROP  (readable_share sh)
          PARAMS (y) GLOBALS (gv)
@@ -98,11 +98,11 @@ Proof.
   destruct left.
   - rewrite sepcon_assoc, (sepcon_comm _ (ghost_var _ _ _)), <- sepcon_assoc.
     erewrite ghost_var_share_join' by eauto with share.
-    Intros; rewrite prop_true_andp by auto; eapply derives_trans, bupd_frame_r; cancel.
-    apply ghost_var_update.
+    Intros; rewrite prop_true_andp by auto; eapply derives_trans, fupd_frame_r; cancel.
+    eapply derives_trans, bupd_fupd; apply ghost_var_update.
   - erewrite sepcon_assoc, ghost_var_share_join' by eauto with share.
-    Intros; rewrite prop_true_andp by auto; eapply derives_trans, bupd_frame_r; cancel.
-    apply ghost_var_update.
+    Intros; rewrite prop_true_andp by auto; eapply derives_trans, fupd_frame_r; cancel.
+    eapply derives_trans, bupd_fupd; apply ghost_var_update.
 Qed.
 #[export] Hint Resolve thread_inv_exclusive : core.
 
@@ -124,11 +124,11 @@ Proof.
     destruct left.
     - rewrite (sepcon_comm _ (ghost_var _ _ _)), <- sepcon_assoc.
       erewrite ghost_var_share_join' by eauto with share.
-      Intros; rewrite prop_true_andp by auto; eapply derives_trans, fupd_frame_r; cancel.
-      eapply derives_trans, bupd_fupd; apply ghost_var_update.
+      Intros; rewrite prop_true_andp by auto; eapply derives_trans, bupd_frame_r; cancel.
+      apply ghost_var_update.
     - erewrite ghost_var_share_join' by eauto with share.
-      Intros; rewrite prop_true_andp by auto; eapply derives_trans, fupd_frame_r; cancel.
-      eapply derives_trans, bupd_fupd; apply ghost_var_update. }
+      Intros; rewrite prop_true_andp by auto; eapply derives_trans, bupd_frame_r; cancel.
+      apply ghost_var_update. }
   Intros; forward_call (gv _ctr_lock, sh, cptr_lock_inv g1 g2 (gv _ctr)).
   { lock_props.
     unfold cptr_lock_inv; Exists (z + 1).
