veric/bi.v
@@ -2,11 +2,11 @@ From iris.bi Require Import interface.
 From iris.proofmode Require Export tactics.
 
 (* undo some "simpl never" settings from std++ *)
-Arguments Pos.of_nat : simpl nomatch.
-Arguments Pos.to_nat !x / .
-Arguments N.add : simpl nomatch.
-Arguments Z.of_nat : simpl nomatch.
-Arguments Z.to_nat : simpl nomatch.
+#[global] Arguments Pos.of_nat : simpl nomatch.
+#[global] Arguments Pos.to_nat !x / .
+#[global] Arguments N.add : simpl nomatch.
+#[global] Arguments Z.of_nat : simpl nomatch.
+#[global] Arguments Z.to_nat : simpl nomatch.
 
 (* Conflicting notations:
 
