Makefile
@@ -739,7 +739,7 @@ hkdf:    _CoqProject $(HKDF_FILES:%.v=sha/%.vo)
 # drbg: _CoqProject $(DRBG_FILES:%.v=verifiedDrbg/%.vo)
 mailbox: _CoqProject mailbox/verif_mailbox_all.vo
 # atomics: _CoqProject atomics/verif_kvnode_atomic.vo atomics/verif_kvnode_atomic_ra.vo atomics/verif_hashtable_atomic.vo atomics/verif_hashtable_atomic_ra.vo
-atomics: _CoqProject atomics/verif_hashtable_atomic.vo $(PROGSDIR)/verif_incr_atomic.vo atomics/lock.vo atomics/verif_lock.vo
+atomics: _CoqProject atomics/verif_hashtable_atomic.vo $(PROGSDIR)/verif_incr_atomic.vo atomics/lock.vo atomics/verif_lock.vo atomics/verif_lock_atomic.vo
 io: _CoqProject $(PROGSDIR)/verif_printf.vo $(PROGSDIR)/verif_io.vo $(PROGSDIR)/verif_io_mem.vo $(PROGSDIR)/io_specs.vo floyd/printf.vo
 
 $(CVOFILES): compcert
